Merge fixes from full-lustre-generalize-frontend-l2nl.

src/Lustre/LSemantics.v
@@ -4,13 +4,18 @@ Open Scope list_scope.
 
 From Coq Require Import Streams.
 From Coq Require Import Sorting.Permutation.
+From Coq Require Import Setoid.
+From Coq Require Import Morphisms.
 
 From Coq Require Import FSets.FMapPositive.
 From Velus Require Import Common.
+From Velus Require Import CommonList.
 From Velus Require Import Environment.
 From Velus Require Import Operators.
 From Velus Require Import Clocks.
 From Velus Require Import Lustre.LSyntax.
+From Velus Require Import Lustre.LOrdered.
+From Velus Require Import NLustre.Streams.
 
 (** * Lustre semantics *)
 
@@ -18,7 +23,8 @@ Module Type LSEMANTICS
        (Import Ids   : IDS)
        (Import Op    : OPERATORS)
        (Import OpAux : OPERATORS_AUX Op)
-       (Import Syn   : LSYNTAX   Ids Op).
+       (Import Syn   : LSYNTAX   Ids Op)
+       (Import Lord  : LORDERED   Ids Op Syn).
 
   (* TODO: put this somewhere else *)
   Infix ":::" := Cons (at level 60, right associativity) : stream_scope.
@@ -81,17 +87,17 @@ Module Type LSEMANTICS
   CoInductive when (k: bool)
                        : Stream value -> Stream value -> Stream value -> Prop :=
   | WhenA:
-      forall xs cs rs,
-        when k xs cs rs ->
+      forall cs xs rs,
+        when k cs xs rs ->
         when k (absent ::: cs) (absent ::: xs) (absent ::: rs)
   | WhenPA:
-      forall x c xs cs rs,
-        when k xs cs rs ->
+      forall c x cs xs rs,
+        when k cs xs rs ->
         val_to_bool c = Some (negb k) ->
         when k (present c ::: cs) (present x ::: xs) (absent ::: rs)
   | WhenPP:
-      forall x c xs cs rs,
-        when k xs cs rs ->
+      forall c x cs xs rs,
+        when k cs xs rs ->
         val_to_bool c = Some k ->
         when k (present c ::: cs) (present x ::: xs) (present x ::: rs).
 
@@ -138,7 +144,12 @@ Module Type LSEMANTICS
   (* TODO: replace idents with (list ident) *)
   Definition idents xs := List.map (@fst ident (type * clock)) xs.
 
-  Notation sem_var H := (fun (x: ident) (s: Stream value) => Env.MapsTo x s H).
+  Inductive sem_var: history -> ident -> Stream value -> Prop :=
+    sem_var_intro:
+      forall H x xs xs',
+        Env.MapsTo x xs' H ->
+        xs ≡ xs' ->
+        sem_var H x xs.
 
   Section NodeSemantics.
 
@@ -147,8 +158,9 @@ Module Type LSEMANTICS
     Inductive sem_exp
                : history -> Stream bool -> exp -> list (Stream value) -> Prop :=
     | Sconst:
-        forall H b c,
-          sem_exp H b (Econst c) [const c b]
+        forall H b c cs,
+          cs ≡ const c b ->
+          sem_exp H b (Econst c) [cs]
 
     | Svar:
         forall H b x s ann,
@@ -221,7 +233,7 @@ Module Type LSEMANTICS
           Forall2 (sem_var H) (idents n.(n_in)) ss ->
           Forall2 (sem_var H) (idents n.(n_out)) os ->
           Forall (sem_equation H b) n.(n_eqs) ->
-          b = sclocksof ss ->
+          b ≡ sclocksof ss ->
           sem_node f ss os.
 
   End NodeSemantics.
@@ -241,8 +253,9 @@ Module Type LSEMANTICS
     Variable P_node : ident -> list (Stream value) -> list (Stream value) -> Prop.
 
     Hypothesis ConstCase:
-      forall H b c,
-        P_exp H b (Econst c) [const c b].
+      forall H b c cs,
+        cs ≡ const c b ->
+        P_exp H b (Econst c) [cs].
 
     Hypothesis VarCase:
       forall H b x s ann,
@@ -328,7 +341,7 @@ Module Type LSEMANTICS
         Forall2 (sem_var H) (idents n.(n_out)) os ->
         Forall (sem_equation G H b) n.(n_eqs) ->
         Forall (P_equation H b) n.(n_eqs) ->
-        b = sclocksof ss ->
+        b ≡ sclocksof ss ->
         P_node f ss os.
 
     Local Ltac SolveForall :=
@@ -357,7 +370,7 @@ Module Type LSEMANTICS
          : P_node f ss os.
     Proof.
       - destruct Sem.
-        + apply ConstCase.
+        + apply ConstCase; eauto.
         + apply VarCase; auto.
         + eapply UnopCase; eauto.
         + eapply BinopCase; eauto.
@@ -375,6 +388,401 @@ Module Type LSEMANTICS
 
   End sem_exp_ind2.
 
+  (** ** Properties of the [global] environment *)
+
+
+  (* TODO: move to CommonList *)
+  Remark In_Forall:
+    forall {A} (x: A) xs P,
+      Forall P xs ->
+      In x xs ->
+      P x.
+  Proof.
+    intros * Hforall Hin.
+    induction xs; inversion Hin; inversion Hforall; subst; auto.
+  Qed.
+
+  Lemma sem_node_cons:
+    forall node G f xs ys,
+      Ordered_nodes (node::G)
+      -> sem_node (node::G) f xs ys
+      -> node.(n_name) <> f
+      -> sem_node G f xs ys.
+  Proof.
+    intros node G f xs ys Hord Hsem Hnf.
+    revert Hnf.
+    induction Hsem using sem_node_ind2
+      with (P_equation := fun bk H eq => ~Is_node_in_eq node.(n_name) eq
+                                      -> sem_equation G bk H eq)
+           (P_exp := fun H bk e ss => ~ Is_node_in_exp node.(n_name) e
+                                   -> sem_exp G H bk e ss);
+      try (now econstructor; eauto).
+    - econstructor; eauto. apply IHHsem.
+      intro. destruct H3. constructor. auto.
+    - econstructor; eauto.
+      apply IHHsem. intro. destruct H5. constructor. auto.
+      apply IHHsem0. intro. destruct H5. constructor. auto.
+    - econstructor; eauto.
+      clear H2 H3 H4. induction H1; eauto. constructor. apply H1.
+      intro. destruct H5. constructor. auto. inv H0.
+      apply IHForall2; eauto. intro. destruct H5. constructor. inv H0.
+      destruct H5; auto.
+      clear H1 H2 H4. induction H3; eauto. constructor. apply H1.
+      intro. destruct H5. constructor. auto.
+      apply IHForall2; eauto. intro. destruct H5. constructor. inv H2.
+      destruct H6; auto.
+    - econstructor; eauto.
+      clear H0 H3. induction H1; eauto. constructor. apply H0.
+      intro. destruct H4. constructor. auto.
+      apply IHForall2; eauto. intro. destruct H4. constructor. inv H3; eauto.
+    - econstructor; eauto.
+      clear H1 H3 H4 H5. induction H2; eauto. constructor. apply H1.
+      intro. destruct H6. constructor. auto.
+      apply IHForall2; eauto. intro. destruct H6. constructor. inv H3.
+      destruct H6; auto.
+      clear H1 H3 H2 H5. induction H4; eauto. constructor. apply H1.
+      intro. destruct H6. constructor. auto.
+      apply IHForall2; eauto. intro. destruct H6. constructor. inv H2.
+      destruct H6; auto.
+    - econstructor; eauto. apply IHHsem.
+      intro. destruct H6. constructor. auto.
+      clear H1 H3 H4 H5. induction H2; eauto. constructor. apply H1.
+      intro. destruct H6. constructor. auto.
+      apply IHForall2; eauto. intro. destruct H6. constructor. inv H3.
+      destruct H6; auto. destruct H3; auto.
+      clear H1 H3 H2 H5. induction H4; eauto. constructor. apply H1.
+      intro. destruct H6. constructor. auto.
+      apply IHForall2; eauto. intro. destruct H6. constructor. inv H2.
+      destruct H6; auto. destruct H2; auto.
+    - inv Hord.
+      econstructor; try apply IHHsem.
+      clear H0 Hsem IHHsem. induction H1; eauto.
+      constructor. apply H0. intro. destruct H2. constructor. auto.
+      apply IHForall2. intro. destruct H2. inv H3. constructor. auto.
+      apply INEapp2.
+      intro. apply H2. rewrite H3. apply INEapp2.
+    - econstructor; eauto.
+      clear H0 H2. induction H1; eauto.
+      constructor. apply H0. intro. destruct H3. now constructor.
+      apply IHForall2. intro. destruct H3. unfold Is_node_in_eq.
+      simpl. Search Exists. rewrite Exists_cons. right. auto.
+    - intro.
+      rewrite find_node_tl with (1:=Hnf) in H0.
+      eapply Snode; eauto.
+      clear H3.
+      eapply Forall_impl_In with (2:=H4).
+      apply find_node_later_not_Is_node_in with (1:=Hord) in H0.
+      intros eq Hin. intro Hini.
+      rewrite Is_node_in_Forall in H0.
+      apply In_Forall with (1:=H0) in Hin.
+      auto.
+  Qed.
+
+  Lemma sem_equation_global_tl:
+    forall nd G H b eq,
+      Ordered_nodes (nd :: G) ->
+      ~ Is_node_in_eq nd.(n_name) eq ->
+      sem_equation (nd :: G) H b eq ->
+      sem_equation G H b eq.
+  Proof.
+    destruct eq as [ xs es ]. intros * Hord Hnin Hsem. inv Hsem.
+
+    econstructor; eauto.
+    clear H6. induction H5 as [ | ? ? ? ? Hsem ]; eauto. constructor.
+
+    clear IHForall2. revert dependent y.
+
+    Ltac SolveNin Hnin :=
+      let Hn := fresh in
+      let Hn2 := fresh in
+      let Hn3 := fresh in
+      let Hn4 := fresh in
+      intro Hn; destruct Hnin; inversion_clear Hn as [? ? Hn2 |]; subst;
+      [ econstructor; econstructor; auto
+      | unfold Is_node_in_eq; simpl; rewrite Exists_cons; right; auto];
+      inversion_clear Hn2 as
+          [ | | ? ? ? ? Hn3 | | ? ? ? ? ? Hn3 | ? ? ? ? ? Hn3 | | ]; auto;
+      try (destruct Hn3 as [| Hn4 ]; eauto; destruct Hn4; eauto).
+
+    induction x using exp_ind2; intros * Hsem; inv Hsem;
+      try (now econstructor; eauto).
+    - econstructor; eauto. eapply IHx; eauto. SolveNin Hnin.
+    - econstructor; eauto.
+      apply IHx1; eauto. SolveNin Hnin.
+      apply IHx2; eauto. SolveNin Hnin.
+    - econstructor; eauto.
+      clear H5 H1 H11 H12. induction H9; auto. constructor.
+      inv H0. apply H4; auto. SolveNin Hnin.
+      inv H0. apply IHForall2; eauto. SolveNin Hnin.
+      clear H5 H0 H9 H12. induction H11; auto. constructor.
+      inv H1. apply H4; auto. SolveNin Hnin.
+      inv H1. apply IHForall2; eauto. SolveNin Hnin.
+    - econstructor; eauto.
+      clear H5 H11 H12. induction H10; eauto. constructor.
+      inv H0. apply H4; eauto. SolveNin Hnin.
+      inv H0. apply IHForall2; eauto. SolveNin Hnin.
+    - econstructor; eauto.
+      clear H5 H1 H10 H13 H14. induction H12; auto. constructor.
+      inv H0. apply H4; auto. SolveNin Hnin.
+      inv H0. apply IHForall2; eauto. SolveNin Hnin.
+      clear H5 H0 H10 H12 H14. induction H13; auto. constructor.
+      inv H1. apply H4; auto. SolveNin Hnin.
+      inv H1. apply IHForall2; eauto. SolveNin Hnin.
+    - econstructor; eauto. eapply IHx; eauto. SolveNin Hnin.
+      clear H5 H1 H10 H13 H14. induction H12; auto. constructor.
+      inv H0. apply H4; auto. SolveNin Hnin.
+      inv H0. apply IHForall2; eauto. SolveNin Hnin.
+      clear H5 H0 H10 H12 H14. induction H13; auto. constructor.
+      inv H1. apply H4; auto. SolveNin Hnin.
+      inv H1. apply IHForall2; eauto. SolveNin Hnin.
+    - econstructor; eauto.
+      clear H5 H10. induction H9; eauto. constructor.
+      inv H0. apply H4; eauto. SolveNin Hnin.
+      inv H0. apply IHForall2; eauto.
+      intro. destruct Hnin. inv H0.
+      inv H3; econstructor. econstructor; eauto. apply INEapp2.
+      unfold Is_node_in_eq; simpl; rewrite Exists_cons; right; auto.
+      eapply sem_node_cons; eauto. intro. destruct Hnin. rewrite H1.
+      econstructor. apply INEapp2.
+    - apply IHForall2. intro. destruct Hnin. unfold Is_node_in_eq. simpl.
+      rewrite Exists_cons. right. auto.
+  Qed.
+
+  Lemma Forall_sem_equation_global_tl:
+    forall nd G b H eqs,
+      Ordered_nodes (nd :: G)
+      -> ~ Is_node_in nd.(n_name) eqs
+      -> Forall (sem_equation (nd :: G) H b) eqs
+      -> Forall (sem_equation G H b) eqs.
+  Proof.
+    intros nd G H b eqs Hord Hnini.
+    apply Forall_impl_In.
+    intros eq Hin Hsem.
+    eapply sem_equation_global_tl; eauto.
+    apply Is_node_in_Forall in Hnini.
+    apply In_Forall with (1:=Hnini) (2:=Hin).
+  Qed.
+
+
+
+
+
+  Add Parametric Morphism v : (fby1 v)
+      with signature @EqSt value ==> @EqSt value ==> @EqSt value ==> Basics.impl
+        as fby1_EqSt.
+  Proof.
+    revert v.
+    cofix Cofix.
+    intros v cs cs' Ecs xs xs' Exs ys ys' Eys H.
+    destruct cs' as [[]], xs' as [[]], ys' as [[]];
+      inv H; inv Ecs; inv Exs; inv Eys; simpl in *;
+        try discriminate.
+    + constructor. eapply Cofix; eauto.
+    + inv H4. econstructor. eapply Cofix; eauto. now inv H2.
+  Qed.
+
+  Add Parametric Morphism : fby
+      with signature @EqSt value ==> @EqSt value ==> @EqSt value ==> Basics.impl
+        as fby_EqSt.
+  Proof.
+    cofix Cofix.
+    intros cs cs' Ecs xs xs' Exs ys ys' Eys H.
+    destruct cs' as [[]], xs' as [[]], ys' as [[]];
+      inv H; inv Ecs; inv Exs; inv Eys; simpl in *;
+        try discriminate.
+    + constructor; eapply Cofix; eauto.
+    + inv H4. inv H. econstructor. inv H2.
+      rewrite <- H1. rewrite <- H3. rewrite <- H5. assumption.
+  Qed.
+
+  Add Parametric Morphism k : (when k)
+      with signature @EqSt value ==> @EqSt value ==> @EqSt value ==> Basics.impl
+        as when_EqSt.
+  Proof.
+    revert k.
+    cofix Cofix.
+    intros k cs cs' Ecs xs xs' Exs ys ys' Eys H.
+    destruct cs' as [[]], xs' as [[]], ys' as [[]];
+      inv H; inv Ecs; inv Exs; inv Eys; simpl in *;
+        try discriminate.
+    + constructor; eapply Cofix; eauto.
+    + constructor. eapply Cofix; eauto. now inv H.
+    + inv H3. inv H5. econstructor. eapply Cofix; eauto. now inv H.
+  Qed.
+
+  Add Parametric Morphism : merge
+      with signature @EqSt value ==> @EqSt value ==>
+                           @EqSt value ==> @EqSt value ==> Basics.impl
+        as merge_EqSt.
+  Proof.
+    cofix Cofix.
+    intros cs cs' Ecs xs xs' Exs ys ys' Eys zs zs' Ezs H.
+    destruct cs' as [[]], xs' as [[]], ys' as [[]], zs' as [[]];
+      inv H; inv Ecs; inv Exs; inv Eys; inv Ezs; simpl in *;
+        try discriminate.
+    + constructor; eapply Cofix; eauto.
+    + inv H. inv H4. inv H6. constructor. eapply Cofix; eauto.
+    + inv H. inv H2. inv H6. constructor. eapply Cofix; eauto.
+  Qed.
+
+  Add Parametric Morphism : ite
+      with signature @EqSt value ==> @EqSt value ==>
+                           @EqSt value ==> @EqSt value ==> Basics.impl
+        as ite_EqSt.
+  Proof.
+    cofix Cofix.
+    intros cs cs' Ecs xs xs' Exs ys ys' Eys zs zs' Ezs H.
+    destruct cs' as [[]], xs' as [[]], ys' as [[]], zs' as [[]];
+      inv H; inv Ecs; inv Exs; inv Eys; inv Ezs; simpl in *;
+        try discriminate.
+    + constructor; eapply Cofix; eauto.
+    + inv H. inv H2. inv H6. constructor; auto. eapply Cofix; eauto.
+    + inv H. inv H4. inv H6. constructor; auto. eapply Cofix; eauto.
+  Qed.
+
+  Add Parametric Morphism op t : (lift1 op t)
+      with signature @EqSt value ==> @EqSt value ==> Basics.impl
+        as lift1_EqSt.
+  Proof.
+    cofix Cofix.
+    intros es es' Ees ys ys' Eys Lift.
+    destruct es' as [[]], ys' as [[]];
+      inv Lift; inv Eys; inv Ees; simpl in *; try discriminate.
+    - constructor; eapply Cofix; eauto.
+    - constructor.
+      + now inv H1; inv H3.
+      + eapply Cofix; eauto.
+  Qed.
+
+  Add Parametric Morphism op t1 t2 : (lift2 op t1 t2)
+      with signature @EqSt value ==> @EqSt value ==> @EqSt value ==> Basics.impl
+        as lift2_EqSt.
+  Proof.
+    cofix Cofix.
+    intros e1s e1s' Ee1s e2s e2s' Ee2s ys ys' Eys Lift.
+    destruct e1s' as [[]], e2s' as [[]], ys' as [[]];
+      inv Lift; inv Eys; inv Ee1s; inv Ee2s; simpl in *; try discriminate.
+    - constructor; eapply Cofix; eauto.
+    - constructor.
+      + now inv H1; inv H3; inv H5.
+      + eapply Cofix; eauto.
+  Qed.
+
+  Add Parametric Morphism c : (const c)
+      with signature @EqSt bool ==> @EqSt value
+        as const_EqSt.
+  Proof.
+    cofix Cofix; intros b b' Eb.
+    unfold_Stv b; unfold_Stv b';
+      constructor; inv Eb; simpl in *; try discriminate; auto.
+  Qed.
+
+  Add Parametric Morphism : sclocksof
+      with signature @EqSts value ==> @EqSt bool
+        as sclocksof_EqSt.
+  Proof.
+    cofix Cofix; intros xs xs' Exs.
+    constructor. simpl.
+    - clear Cofix.
+      revert dependent xs'.
+      induction xs; intros; try inv Exs; simpl; auto.
+      f_equal; auto.
+      now rewrite H1.
+    - apply Cofix.
+      clear Cofix.
+      revert dependent xs'.
+      induction xs; intros; try inv Exs; simpl; constructor.
+      + now rewrite H1.
+      + now apply IHxs.
+  Qed.
+
+  Add Parametric Morphism H : (sem_var H)
+      with signature eq ==> @EqSt value ==> Basics.impl
+        as sem_var_EqSt.
+  Proof.
+    intros x xs xs' E; intro Sem; inv Sem.
+    econstructor; eauto.
+    Show Proof.
+    transitivity xs; auto; symmetry; auto.
+  Qed.
+
+  Add Parametric Morphism G : (sem_node G)
+      with signature eq ==> @EqSts value ==> @EqSts value ==> Basics.impl
+        as mod_sem_node_morph.
+  Proof.
+    unfold Basics.impl; intros f xss xss' Exss yss yss' Eyss Sem.
+    induction Sem.
+    econstructor; eauto.
+    + now rewrite <-Exss.
+    + now rewrite <-Eyss.
+    + now rewrite Exss in H4.
+  Qed.
+
+  Add Parametric Morphism G H : (sem_exp G H)
+      with signature @EqSt bool ==> eq ==> @EqSts value ==> Basics.impl
+        as sem_exp_morph.
+  Proof.
+    intros b b' Eb e xs xs' Exs Sem.
+    revert b' xs' Eb Exs; induction Sem using sem_exp_ind2 with
+                              (P_equation := fun H b e => True)
+                              (P_node := fun i ls xs => True).
+    - intros. inv Exs. inv H5.
+      constructor.
+      rewrite <-Eb.
+      transitivity cs; auto.
+      now symmetry.
+    - intros. inv Exs. inv H5.
+      econstructor; eauto.
+      eapply sem_var_EqSt; eauto.
+    - intros. inv Exs. inv H6.
+      econstructor; eauto.
+      apply IHSem; auto; try reflexivity.
+      now rewrite <- H4.
+    - intros. inv Exs. inv H7.
+      econstructor; eauto.
+      + apply IHSem1; auto; reflexivity.
+      + apply IHSem2; auto; reflexivity.
+      + now rewrite <- H5.
+    - intros.
+      econstructor.
+      + instantiate (1 := s0ss).
+        eapply Forall2_impl_In; [ idtac | apply H1 ].
+        simpl. intros. apply H7; eauto. reflexivity.
+      + instantiate (1 := sss).
+        eapply Forall2_impl_In; [ idtac | apply H3 ].
+        simpl. intros. apply H7; eauto. reflexivity.
+      + eapply Forall3_EqSt; eauto. solve_proper.
+    - intros. econstructor; eauto.
+      + instantiate (1 := ss).
+        eapply Forall2_impl_In; [ idtac | apply H1 ].
+        simpl. intros. apply H6; eauto. reflexivity.
+      + eapply Forall2_EqSt; eauto. solve_proper.
+    - intros. econstructor; eauto.
+      + instantiate (1 := ts).
+        eapply Forall2_impl_In; [ idtac | apply H2 ].
+        simpl. intros. apply H8; eauto. reflexivity.
+      + instantiate (1 := fs).
+        eapply Forall2_impl_In; [ idtac | apply H4 ].
+        simpl. intros. apply H8; eauto. reflexivity.
+      + eapply Forall3_EqSt; eauto. solve_proper.
+    - intros. econstructor; eauto.
+      + eapply IHSem; eauto. reflexivity.
+      + instantiate (1 := ts).
+        eapply Forall2_impl_In; [ idtac | apply H1 ].
+        simpl. intros. apply H7; eauto. reflexivity.
+      + instantiate (1 := fs).
+        eapply Forall2_impl_In; [ idtac | apply H3 ].
+        simpl. intros. apply H7; eauto. reflexivity.
+      + eapply Forall3_EqSt; eauto. solve_proper.
+    - intros. econstructor.
+      + instantiate (1 := ss).
+        eapply Forall2_impl_In; [ idtac | apply H1 ].
+        intros. simpl. apply H5; auto. reflexivity.
+      + now rewrite <- Exs.
+    - split.
+    - split.
+  Qed.
+
 End LSEMANTICS.
 
 Module LSemanticsFun
@@ -382,6 +790,7 @@ Module LSemanticsFun
        (Import Op    : OPERATORS)
        (Import OpAux : OPERATORS_AUX Op)
        (Import Syn   : LSYNTAX   Ids Op)
-       <: LSEMANTICS Ids Op OpAux Syn.
-  Include LSEMANTICS Ids Op OpAux Syn.
+       (Import Lord  : LORDERED  Ids Op Syn)
+       <: LSEMANTICS Ids Op OpAux Syn Lord.
+  Include LSEMANTICS Ids Op OpAux Syn Lord.
 End LSemanticsFun.
