src/Lustre/LOrdered.v
@@ -1,0 +1,169 @@
+From Coq Require Import PArith.
+From Coq Require Import List.
+Import List.ListNotations.
+Open Scope list_scope.
+
+From Velus Require Import Common.
+From Velus Require Import Operators.
+From Velus Require Import Clocks.
+From Velus Require Import Lustre.LSyntax.
+
+(** * Ordering of Lustre nodes *)
+
+(**
+
+The compilation of a whole program is only correct if that program satisfies
+the [Ordered_nodes] predicate, which states that a node may only call nodes
+that were defined earlier.
+
+ *)
+
+Module Type LORDERED
+       (Ids         : IDS)
+       (Op          : OPERATORS)
+       (Import Syn  : LSYNTAX Ids Op).
+
+  Inductive Is_node_in_exp : ident -> exp -> Prop :=
+  | INEunop: forall f op e a,
+      Is_node_in_exp f e -> Is_node_in_exp f (Eunop op e a)
+  | INEbinop: forall f op e1 e2 a,
+      Is_node_in_exp f e1 \/ Is_node_in_exp f e2 ->
+      Is_node_in_exp f (Ebinop op e1 e2 a)
+  | INEfby: forall f le1 le2 la,
+      Exists (Is_node_in_exp f) le1 \/ Exists (Is_node_in_exp f) le2 ->
+      Is_node_in_exp f (Efby le1 le2 la)
+  | INEwhen: forall f le x b la,
+      Exists (Is_node_in_exp f) le ->
+      Is_node_in_exp f (Ewhen le x b la)
+  | INEmerge: forall f x le1 le2 la,
+      Exists (Is_node_in_exp f) le1 \/ Exists (Is_node_in_exp f) le2 ->
+      Is_node_in_exp f (Emerge x le1 le2 la)
+  | INEite: forall f e le1 le2 la,
+      Is_node_in_exp f e
+      \/ Exists (Is_node_in_exp f) le1
+      \/ Exists (Is_node_in_exp f) le2 ->
+      Is_node_in_exp f (Eite e le1 le2 la)
+  | INEapp1: forall f g le a,
+      Exists (Is_node_in_exp f) le ->
+      Is_node_in_exp f (Eapp g le a)
+  | INEapp2: forall f le a, Is_node_in_exp f (Eapp f le a).
+
+  Definition Is_node_in_eq (f: ident) (eq: equation) : Prop :=
+    List.Exists (Is_node_in_exp f) (snd eq).
+
+  (* definition is needed in signature *)
+  Definition Is_node_in (f: ident) (eqs: list equation) : Prop :=
+    List.Exists (Is_node_in_eq f) eqs.
+
+  Inductive Ordered_nodes : global -> Prop :=
+  | ONnil: Ordered_nodes nil
+  | ONcons:
+      forall nd nds,
+        Ordered_nodes nds
+        -> (forall f, Is_node_in f nd.(n_eqs) ->
+                f <> nd.(n_name)
+                /\ List.Exists (fun n=> f = n.(n_name)) nds)
+        -> List.Forall (fun nd'=> nd.(n_name) <> nd'.(n_name))%type nds
+        -> Ordered_nodes (nd::nds).
+
+  (** ** Properties of [Is_node_in] *)
+
+  Section Is_node_Properties.
+
+    Lemma not_Is_node_in_cons:
+      forall n eq eqs,
+        ~ Is_node_in n (eq::eqs) <-> ~Is_node_in_eq n eq /\ ~Is_node_in n eqs.
+    Proof.
+      intros n eq eqs.
+      split; intro HH.
+      - split; intro; apply HH; unfold Is_node_in; intuition.
+      - destruct HH; inversion_clear 1; intuition.
+    Qed.
+
+    Lemma Is_node_in_Forall:
+      forall n eqs,
+        ~Is_node_in n eqs <-> List.Forall (fun eq=>~Is_node_in_eq n eq) eqs.
+    Proof.
+      induction eqs as [|eq eqs IH];
+      [split; [now constructor|now inversion 2]|].
+      split; intro HH.
+      - apply not_Is_node_in_cons in HH.
+        destruct HH as [Heq Heqs].
+        constructor; [exact Heq|apply IH with (1:=Heqs)].
+      - apply not_Is_node_in_cons.
+        inversion_clear HH as [|? ? Heq Heqs].
+        apply IH in Heqs.
+        intuition.
+    Qed.
+
+  End Is_node_Properties.
+
+  (** ** Properties of [Ordered_nodes] *)
+
+  Section Ordered_nodes_Properties.
+
+    Lemma Ordered_nodes_append:
+      forall G G',
+        Ordered_nodes (G ++ G')
+        -> Ordered_nodes G'.
+    Proof.
+      induction G as [|nd G IH]; [intuition|].
+      intros G' HnGG.
+      apply IH; inversion_clear HnGG; assumption.
+    Qed.
+
+    Lemma find_node_later_not_Is_node_in:
+      forall f nd G nd',
+        Ordered_nodes (nd::G)
+        -> find_node f G = Some nd'
+        -> ~Is_node_in nd.(n_name) nd'.(n_eqs).
+    Proof.
+      intros f nd G nd' Hord Hfind Hini.
+      apply find_node_split in Hfind.
+      destruct Hfind as [bG [aG HG]].
+      rewrite HG in Hord.
+      inversion_clear Hord as [|? ? Hord' H0 Hnin]; clear H0.
+      apply Ordered_nodes_append in Hord'.
+      inversion_clear Hord' as [| ? ? Hord Heqs Hnin'].
+      apply Heqs in Hini.
+      destruct Hini as [H0 HH]; clear H0.
+      rewrite Forall_app in Hnin.
+      destruct Hnin as [H0 Hnin]; clear H0.
+      inversion_clear Hnin as [|? ? H0 HH']; clear H0.
+      apply List.Exists_exists in HH.
+      destruct HH as [node [HaG Heq]].
+      rewrite List.Forall_forall in HH'.
+      apply HH' in HaG.
+      contradiction.
+    Qed.
+
+    Lemma find_node_not_Is_node_in:
+      forall f nd G,
+        Ordered_nodes G
+        -> find_node f G = Some nd
+        -> ~Is_node_in nd.(n_name) nd.(n_eqs).
+    Proof.
+      intros f nd G Hord Hfind.
+      apply find_node_split in Hfind.
+      destruct Hfind as [bG [aG HG]].
+      rewrite HG in Hord.
+      apply Ordered_nodes_append in Hord.
+      inversion_clear Hord as [|? ? Hord' Heqs Hnin].
+      intro Hini.
+      apply Heqs in Hini.
+      destruct Hini as [HH H0]; clear H0.
+      apply HH; reflexivity.
+    Qed.
+
+  End Ordered_nodes_Properties.
+
+End LORDERED.
+
+Module LOrderedFun
+       (Ids  : IDS)
+       (Op   : OPERATORS)
+       (Syn  : LSYNTAX Ids Op)
+       <: LORDERED Ids Op Syn.
+  Include LORDERED Ids Op Syn.
+End LOrderedFun.
+
