src/Lustre/Lustre.v
@@ -4,6 +4,7 @@ From Velus Require Export Lustre.LSyntax.
 From Velus Require Export Lustre.LClocking.
 From Velus Require Export Lustre.LTyping.
 From Velus Require Export Lustre.LSemantics.
+From Velus Require Export Lustre.LOrdered.
 
 From Velus Require Import Common.
 
@@ -14,7 +15,8 @@ Module Type LUSTRE
   Declare Module Export Syn: LSYNTAX    Ids Op.
   Declare Module Export Typ: LTYPING    Ids Op       Syn.
   Declare Module Export Clo: LCLOCKING  Ids Op       Syn.
-  Declare Module Export Sem: LSEMANTICS Ids Op OpAux Syn.
+  Declare Module Export Lord: LORDERED  Ids Op       Syn.
+  Declare Module Export Sem: LSEMANTICS Ids Op OpAux Syn Lord.
 End LUSTRE.
 
 Module LustreFun
@@ -25,6 +27,7 @@ Module LustreFun
   Module Export Syn := LSyntaxFun     Ids Op.
   Module Export Typ := LTypingFun     Ids Op       Syn.
   Module Export Clo := LClockingFun   Ids Op       Syn.
-  Module Export Sem := LSemanticsFun  Ids Op OpAux Syn.
+  Module Export Lord:= LOrderedFun    Ids Op       Syn.
+  Module Export Sem := LSemanticsFun  Ids Op OpAux Syn Lord.
 End LustreFun.
 
